PiLL/PiLL/Alt.lean
@@ -2,113 +2,6 @@ import Mathlib.Data.Finset.Basic
 import Mathlib.Data.Finset.Card
 import Mathlib.Data.Finset.Fold
 
-
-/- Original working example -/
--- abbrev PName := Nat
-
--- inductive Proc : Type where
---   | tensor  (x y : PName) (P : Proc)
---   | parr    (x y : PName) (P : Proc)
---   | one     (x : PName) (P : Proc)
---   | bot     (x : PName) (P : Proc)
---   | cut     (x y : PName) (P : Proc)
---   | par     (P Q : Proc)
---   | nil
--- deriving DecidableEq
-
--- abbrev Atom := Nat
-
--- inductive Types : Type where
---   | atom      (a : Atom)
---   | atomDual  (a : Atom)
---   | tensor    (A B : Types)
---   | parr      (A B : Types)
---   | one
---   | bot
--- deriving DecidableEq
-
--- abbrev Env := Finset (PName × Types)
-
--- abbrev HyperEnv := Finset (Env)
-
--- inductive Act : Type
---   | one     (x : PName)
---   | bot     (x : PName)
---   | tensor  (x y : PName)
---   | parr    (x y : PName)
--- deriving Repr, DecidableEq
-
--- inductive Lbl : Type
---   | tau
---   | act   (a : Act)
---   | par   (l l' : Act)
--- deriving Repr, DecidableEq
-
--- theorem swap_last (Γ Δ Ξ : Env) : Γ ∪ Δ ∪ Ξ = Γ ∪ Ξ ∪ Δ := by
---   rw [Finset.union_assoc, Finset.union_comm Δ Ξ, Finset.union_assoc]
-
--- inductive Typing : HyperEnv → Proc → Prop where
---   | bot {Γ : Env} {P : Proc} {x : PName} {A : Types} :
---       Typing {Γ} P →
---       Typing {Γ ∪ {(x, Types.bot)}} (Proc.bot x P)
-
---   | parr {Γ : Env} {P : Proc} {x y : PName} {A B : Types} :
---       Typing {Γ ∪ {(y, A)} ∪ {(x, B)}} P →
---       Typing {Γ ∪ {(x, A.parr B)}} (Proc.parr x y P)
-
--- inductive TypingStep : HyperEnv → Proc → Lbl →
---   HyperEnv → Proc → Prop where
---    | bot
---       {Γ : Env} {P : Proc} {x : Nat }
---       (𝒟 : Typing {Γ ∪ {(x, Types.bot)}} (Proc.bot x P))
---       (𝒟' : Typing {Γ} P) :
---       TypingStep
---         {Γ ∪ {(x, Types.bot)}} (Proc.bot x P)
---         (Lbl.act (Act.bot x))
---         {Γ} P
-
---   | parr
---       {Γ : Env} {P : Proc} {x y : Nat} {A B : Types}
---       (𝒟 : Typing {Γ ∪ {(x, A.parr B)}} (Proc.parr x y P))
---       (𝒟' : Typing {Γ ∪ {(y, A)} ∪ {(x, B)}} P) :
---       TypingStep
---         {Γ ∪ {(x, A.parr B)}} (Proc.parr x y P)
---         (Lbl.act (Act.parr x y))
---         {Γ ∪ {(y, A)} ∪ {(x, B)}} P
-
-
--- example (Γ : Env) (P : Proc) (x y z : PName) (A B : Types)
---   (h : Typing {Γ ∪ ({(y, A)} ∪ {(x, B)})} P) :
---   TypingStep
---     {Γ ∪ {(x, A.parr B)} ∪ {(z, Types.bot)}} (Proc.parr x y (Proc.bot z P))
---     (Lbl.act (Act.parr x y))
---     {Γ ∪ {(y, A)} ∪ {(x, B)} ∪ {(z, Types.bot)}} (Proc.bot z P) := by
-
---   have h1 : (Γ ∪ {(x, A.parr B)} ∪ {(z, Types.bot)}) =
---     (Γ ∪ {(z, Types.bot)} ∪ {(x, A.parr B)}) := by rw [swap_last]
-
---   have h2 : (Γ ∪ {(y, A)} ∪ {(x, B)} ∪ {(z, Types.bot)}) =
---     (Γ ∪ {(z, Types.bot)}) ∪ {(y, A)} ∪ {(x, B)} := by
---     conv => lhs ; lhs ; rw [Finset.union_assoc]
---     rw [swap_last, ← Finset.union_assoc]
-
---   rw [h1, h2]
---   apply TypingStep.parr
---   · apply Typing.parr
---     rw [Finset.union_assoc, swap_last]
---     apply Typing.bot
---     · simp_all only [Finset.union_singleton]
---       exact A
---     · exact h
---   · rw [Finset.union_assoc, swap_last]
---     · apply Typing.bot
---       · simp_all only [Finset.union_singleton]
---         exact A
---       · exact h
-
-/- End of original working example -/
-
-
 abbrev PName := Nat
 
 inductive Proc : Type where
@@ -155,10 +48,8 @@ theorem swap_last (A B C : Env) : A ∪ B ∪ C = A ∪ C ∪ B := by
 theorem move_last_two_forward (A B C D : Env) : ((A ∪ B) ∪ C) ∪ D = ((A ∪ D) ∪ B) ∪ C := by
   rw [Finset.union_assoc A B C, swap_last, ← Finset.union_assoc]
 
-
-/- Slight modification of original which also works -/
 inductive Typing : HyperEnv → Proc → Prop where
-  | bot {Γ : Env} {P : Proc} {x : PName} {A : Types} :
+  | bot {Γ : Env} {P : Proc} {x : PName} : -- {A : Types} :
       Typing {Γ} P →
       Typing {Γ ∪ {(x, Types.bot)}} (Proc.bot x P)
 
@@ -202,122 +93,141 @@ example {Γ : Env} {P : Proc} {x y z : PName} {A B : Types}
     exact 𝒟'
 
 
-/- Does not work, whenever I try and wrap HyperEnv and Proc into a Typing then
-   for some reason the motive isn't type correct -/
-inductive Typing_ALT : HyperEnv → Proc → Prop where
-  | bot {Γ : Env} {P : Proc} {x : PName} {A : Types} :
-      Typing_ALT {Γ} P →
-      Typing_ALT {Γ ∪ {(x, Types.bot)}} (Proc.bot x P)
 
-  | parr {Γ : Env} {P : Proc} {x y : PName} {A B : Types} :
-      Typing_ALT {Γ ∪ {(y, A)} ∪ {(x, B)}} P →
-      Typing_ALT {Γ ∪ {(x, A.parr B)}} (Proc.parr x y P)
 
-inductive TypingStep_ALT : ∀ {𝒢 𝒢' : HyperEnv} {P P' : Proc},
-  Typing_ALT 𝒢 P → Lbl → Typing_ALT 𝒢' P' → Prop where
-  | bot
-      {Γ : Env} {P : Proc} {x : Nat}
-      (𝒟 : Typing_ALT {Γ ∪ {(x, Types.bot)}} (Proc.bot x P))
-      (𝒟' : Typing_ALT {Γ} P) :
-      TypingStep_ALT 𝒟 (Lbl.act (Act.bot x)) 𝒟'
-
-  | parr
-      {Γ : Env} {P : Proc} {x y : Nat} {A B : Types}
-      (𝒟 : Typing_ALT {Γ ∪ {(x, A.parr B)}} (Proc.parr x y P))
-      (𝒟' : Typing_ALT {Γ ∪ {(y, A)} ∪ {(x, B)}} P) :
-      TypingStep_ALT 𝒟 (Lbl.act (Act.parr x y)) 𝒟'
-
-example {Γ : Env} {P : Proc} {x y z : PName} {A B : Types}
-  (𝒟 : Typing_ALT {Γ ∪ {(y, A.parr B)} ∪ {(z, Types.bot)}} (Proc.parr x y (Proc.bot z P)))
-  (𝒟' : Typing_ALT {Γ ∪ {(y, A)} ∪ {(x, B)} ∪ {(z, Types.bot)}} (Proc.bot z P)) :
-  TypingStep_ALT
-    𝒟
-    (Lbl.act (Act.parr x y))
-    𝒟' := by
-    sorry
-  -- rw [swap_last] at 𝒟 -- creates copy
-  -- rw [move_last_two_forward] at 𝒟' -- creates copy
-  -- rw [swap_last, move_last_two_forward] -- motive error
-  -- apply TypingStep_ALT.parr
-  -- · rw [← swap_last]
-  --   exact 𝒟
-  -- · rw [← move_last_two_forward]
-  --   exact 𝒟'
 
 /- WIP: Small extension to TypingStep trying to get the execution in example 2.5 to work -/
-inductive TypingStep_extended : HyperEnv → Proc → Lbl →
-  HyperEnv → Proc → Prop where
-   | bot
-      {Γ : Env} {P : Proc} {x : Nat}
-      (𝒟 : Typing {Γ ∪ {(x, Types.bot)}} (Proc.bot x P))
-      (𝒟' : Typing {Γ} P) :
-      TypingStep_extended
-        {Γ ∪ {(x, Types.bot)}} (Proc.bot x P)
-        (Lbl.act (Act.bot x))
-        {Γ} P
+-- inductive TypingStep_extended : HyperEnv → Proc → Lbl →
+--   HyperEnv → Proc → Prop where
+--    | bot
+--       {Γ : Env} {P : Proc} {x : Nat}
+--       (𝒟 : Typing {Γ ∪ {(x, Types.bot)}} (Proc.bot x P))
+--       (𝒟' : Typing {Γ} P) :
+--       TypingStep_extended
+--         {Γ ∪ {(x, Types.bot)}} (Proc.bot x P)
+--         (Lbl.act (Act.bot x))
+--         {Γ} P
 
-  | parr
-      {Γ : Env} {P : Proc} {x y : Nat} {A B : Types}
-      (𝒟 : Typing {Γ ∪ {(x, A.parr B)}} (Proc.parr x y P))
-      (𝒟' : Typing {Γ ∪ {(y, A)} ∪ {(x, B)}} P) :
-      TypingStep_extended
-        {Γ ∪ {(x, A.parr B)}} (Proc.parr x y P)
-        (Lbl.act (Act.parr x y))
-        {Γ ∪ {(y, A)} ∪ {(x, B)}} P
+--   | parr
+--       {Γ : Env} {P : Proc} {x y : Nat} {A B : Types}
+--       (𝒟 : Typing {Γ ∪ {(x, A.parr B)}} (Proc.parr x y P))
+--       (𝒟' : Typing {Γ ∪ {(y, A)} ∪ {(x, B)}} P) :
+--       TypingStep_extended
+--         {Γ ∪ {(x, A.parr B)}} (Proc.parr x y P)
+--         (Lbl.act (Act.parr x y))
+--         {Γ ∪ {(y, A)} ∪ {(x, B)}} P
 
-  | syn
-      {𝒢 𝒢' ℋ ℋ' : HyperEnv} {P P' Q Q' : Proc} {a a' : Act}
-      {𝒟 : Typing 𝒢 P} {𝒟' : Typing 𝒢' P'}
-      {ℰ : Typing ℋ Q} {ℰ' : Typing ℋ' Q'}
-      (h₁ : TypingStep_extended 𝒢 P (Lbl.act a) 𝒢' P')
-      (h₂ : TypingStep_extended ℋ Q (Lbl.act a') ℋ' Q')
-      -- (disj : ((Lbl.par a a').iNames ∩ (Proc.par P Q).fNames) = ∅)
-      :
-      ----------------------------------------------------------------------
-      TypingStep_extended (𝒢 ∪ ℋ) (P.par Q) (Lbl.par a a') (𝒢' ∪ ℋ') (P'.par Q')
+--   | syn
+--       {𝒢 𝒢' ℋ ℋ' : HyperEnv} {P P' Q Q' : Proc} {a a' : Act}
+--       {𝒟 : Typing 𝒢 P} {𝒟' : Typing 𝒢' P'}
+--       {ℰ : Typing ℋ Q} {ℰ' : Typing ℋ' Q'}
+--       (h₁ : TypingStep_extended 𝒢 P (Lbl.act a) 𝒢' P')
+--       (h₂ : TypingStep_extended ℋ Q (Lbl.act a') ℋ' Q')
+--       -- (disj : ((Lbl.par a a').iNames ∩ (Proc.par P Q).fNames) = ∅)
+--       :
+--       ----------------------------------------------------------------------
+--       TypingStep_extended (𝒢 ∪ ℋ) (P.par Q) (Lbl.par a a') (𝒢' ∪ ℋ') (P'.par Q')
 
-  | tensor
-      {Γ Δ : Env} {P : Proc} {x y : Nat} {A B : Types}
-      {𝒟 : Typing {Γ ∪ Δ ∪ {(x, A.tensor B)}} (Proc.tensor x y P)}
-      {𝒟' : Typing ({Γ ∪ {(y, A)}} ∪ {Δ ∪ {(x, B)}}) P} :
-      TypingStep_extended
-        {Γ ∪ Δ ∪ {(x, A.tensor B)}} (Proc.tensor x y P)
-        (Lbl.act (Act.tensor x y))
-        ({Γ ∪ {(y, A)}} ∪ {Δ ∪ {(x, B)}}) P
+--   | tensor
+--       {Γ Δ : Env} {P : Proc} {x y : Nat} {A B : Types}
+--       {𝒟 : Typing {Γ ∪ Δ ∪ {(x, A.tensor B)}} (Proc.tensor x y P)}
+--       {𝒟' : Typing ({Γ ∪ {(y, A)}} ∪ {Δ ∪ {(x, B)}}) P} :
+--       TypingStep_extended
+--         {Γ ∪ Δ ∪ {(x, A.tensor B)}} (Proc.tensor x y P)
+--         (Lbl.act (Act.tensor x y))
+--         ({Γ ∪ {(y, A)}} ∪ {Δ ∪ {(x, B)}}) P
 
 /-
   SYN, ⊗, ⅋ part of the tau transition of the execution in example 2.5
   the CUT part is still missing.
 -/
-example {Γ Γ' Δ : Env} {Q R : Proc} {x x' y y' z : PName} {A B A' B' : Types}
-  (𝒟 : Typing
-        ({Γ' ∪ Γ ∪ {(x, A.tensor B)}} ∪ {Δ ∪ {(y, A'.parr B')} ∪ {(z, Types.bot)}})
-        (Proc.par (Proc.tensor x x' Q) (Proc.parr y y' (Proc.bot z R))))
-  (𝒟' : Typing
-        ({Γ' ∪ {(x', A)}} ∪ {Γ ∪ {(x, B)}} ∪ {Δ ∪ {(y', A')} ∪ {(y, B')} ∪ {(z, Types.bot)}})
-        (Proc.par (Q) (Proc.bot z R)))
+-- example {Γ Γ' Δ : Env} {Q R : Proc} {x x' y y' z : PName} {A B A' B' : Types}
+--   (𝒟 : Typing
+--         ({Γ' ∪ Γ ∪ {(x, A.tensor B)}} ∪ {Δ ∪ {(y, A'.parr B')} ∪ {(z, Types.bot)}})
+--         (Proc.par (Proc.tensor x x' Q) (Proc.parr y y' (Proc.bot z R))))
+--   (𝒟' : Typing
+--         ({Γ' ∪ {(x', A)}} ∪ {Γ ∪ {(x, B)}} ∪ {Δ ∪ {(y', A')} ∪ {(y, B')} ∪ {(z, Types.bot)}})
+--         (Proc.par (Q) (Proc.bot z R)))
 
-  (ℰ : Typing {Γ' ∪ Γ ∪ {(x, A.tensor B)}} (Proc.tensor x x' Q))
-  (ℰ' : Typing ({Γ' ∪ {(x', A)}} ∪ {Γ ∪ {(x, B)}}) Q)
-  (ℱ : Typing {Δ ∪ {(y, A'.parr B')} ∪ {(z, Types.bot)}} (Proc.parr y y' (Proc.bot z R)))
-  (ℱ'' : Typing {Δ ∪ {(y', A')} ∪ {(y, B')} ∪ {(z, Types.bot)}} (Proc.bot z R)) :
-  TypingStep_extended
-    ({Γ' ∪ Γ ∪ {(x, A.tensor B)}} ∪ {Δ ∪ {(y, A'.parr B')} ∪ {(z, Types.bot)}})
-    (Proc.par (Proc.tensor x x' Q) (Proc.parr y y' (Proc.bot z R)))
-    (Lbl.par (Act.tensor x x') (Act.parr y y'))
-    ({Γ' ∪ {(x', A)}} ∪ {Γ ∪ {(x, B)}} ∪ {Δ ∪ {(y', A')} ∪ {(y, B')} ∪ {(z, Types.bot)}})
-    (Proc.par (Q) (Proc.bot z R)) := by
-    apply TypingStep_extended.syn
-    · exact ℰ
-    · exact ℰ'
-    · exact ℱ
-    · exact ℱ''
-    · apply TypingStep_extended.tensor
-      · exact ℰ
-      · exact ℰ'
-    · rw [swap_last, move_last_two_forward]
-      · apply TypingStep_extended.parr
-        · rw [← swap_last]
-          exact ℱ
-        · rw [← move_last_two_forward]
-          exact ℱ''
+--   (ℰ : Typing {Γ' ∪ Γ ∪ {(x, A.tensor B)}} (Proc.tensor x x' Q))
+--   (ℰ' : Typing ({Γ' ∪ {(x', A)}} ∪ {Γ ∪ {(x, B)}}) Q)
+--   (ℱ : Typing {Δ ∪ {(y, A'.parr B')} ∪ {(z, Types.bot)}} (Proc.parr y y' (Proc.bot z R)))
+--   (ℱ'' : Typing {Δ ∪ {(y', A')} ∪ {(y, B')} ∪ {(z, Types.bot)}} (Proc.bot z R)) :
+--   TypingStep_extended
+--     ({Γ' ∪ Γ ∪ {(x, A.tensor B)}} ∪ {Δ ∪ {(y, A'.parr B')} ∪ {(z, Types.bot)}})
+--     (Proc.par (Proc.tensor x x' Q) (Proc.parr y y' (Proc.bot z R)))
+--     (Lbl.par (Act.tensor x x') (Act.parr y y'))
+--     ({Γ' ∪ {(x', A)}} ∪ {Γ ∪ {(x, B)}} ∪ {Δ ∪ {(y', A')} ∪ {(y, B')} ∪ {(z, Types.bot)}})
+--     (Proc.par (Q) (Proc.bot z R)) := by
+--     apply TypingStep_extended.syn
+--     · exact ℰ
+--     · exact ℰ'
+--     · exact ℱ
+--     · exact ℱ''
+--     · apply TypingStep_extended.tensor
+--       · exact ℰ
+--       · exact ℰ'
+--     · rw [swap_last, move_last_two_forward]
+--       · apply TypingStep_extended.parr
+--         · rw [← swap_last]
+--           exact ℱ
+--         · rw [← move_last_two_forward]
+--           exact ℱ''
+
+
+
+/- Zulip example -/
+-- abbrev Env := Finset (Nat × Nat)
+-- abbrev HyperEnv := Finset (Env)
+
+-- inductive Typing : HyperEnv → Prop where
+--   | parr {Γ : Env} {x y A B : Nat} :
+--       Typing {Γ ∪ {(y, A)} ∪ {(x, B)}} →
+--       Typing {Γ ∪ {(x, A + B)}}
+
+-- inductive TS1 : HyperEnv → List (Nat × Nat) →
+--   HyperEnv → Prop where
+--   | parr
+--       {Γ : Env} {x y A B : Nat}
+--       (𝒟 : Typing {Γ ∪ {(x, A + B)}})
+--       (𝒟' : Typing {Γ ∪ {(y, A)} ∪ {(x, B)}}) :
+--       TS1
+--         {Γ ∪ {(x, A + B)}}
+--         [(x, y)]
+--         {Γ ∪ {(y, A)} ∪ {(x, B)}}
+
+-- inductive TS2 : ∀ {𝒢 𝒢' : HyperEnv},
+--   Typing 𝒢 → List (Nat × Nat) → Typing 𝒢' → Prop where
+--   | parr
+--       {Γ : Env} {x y A B : Nat}
+--       (𝒟 : Typing {Γ ∪ {(y, A)} ∪ {(x, B)}}) :
+--       TS2
+--         (Typing.parr 𝒟)
+--         [(x, y)]
+--         𝒟
+
+-- theorem swap_last_two (A B C : Env) : A ∪ B ∪ C = A ∪ C ∪ B := by aesop
+-- theorem move_last_two_left (A B C D : Env) : A ∪ B ∪ C ∪ D = A ∪ D ∪ B ∪ C := by aesop
+
+-- theorem example1 {Γ : Env} {x y z A B : Nat}
+--   (𝒟 : Typing {Γ ∪ {(x, A + B)} ∪ {(z, 0)}})
+--   (𝒟' : Typing {Γ ∪ {(y, A)} ∪ {(x, B)} ∪ {(z, 0)}}) :
+--   TS1
+--     {Γ ∪ {(x, A + B)} ∪ {(z, 0)}}
+--     [(x, y)]
+--     {Γ ∪ {(y, A)} ∪ {(x, B)} ∪ {(z, 0)}} := by
+--   rw [move_last_two_left]
+--   rw [swap_last_two]
+--   apply TS1.parr
+--   · rw [← swap_last_two] ; exact 𝒟
+--   · rw [← move_last_two_left] ; exact 𝒟'
+
+-- theorem example2 {Γ : Env} {x y z A B : Nat}
+--   (𝒟 : Typing {Γ ∪ {(y, A)} ∪ {(x, B)} ∪ {(z, 0)}}) :
+--   TS2
+--     (Typing.parr 𝒟)
+--     [(x, y)]
+--     𝒟 := by
+--   rw [swap_last_two] at 𝒟 -- Creates a copy instead of rewriting the goal
+--   rw [move_last_two_left] -- Tactic `rewrite` failed: motive is not type correct
+--   sorry
